src2/Typing.v
@@ -10,7 +10,6 @@ From Coq Require Import
 From Heapster2 Require Import
      Utils
      Permissions
-     PermissionsSpred2
      SepStep.
 
 From ExtLib Require Import
@@ -62,124 +61,107 @@ Qed.
 (** * Stuttering bisimulation *)
 Section bisim.
   Context {config specConfig : Type}.
-  Context {Spred : Type}.
-  Context {interp_spred : Spred -> config * specConfig -> Prop}.
 
-  Inductive bisim_gen {R1 R2 : Type}
-            (bisim : forall (spred : Spred),
-                @perm {x | interp_spred spred x} ->
-                (R1 -> R2 -> Perms2) ->
-                itree (sceE config) R1 ->
-                config ->
-                itree (sceE specConfig) R2 ->
-                specConfig ->
-                Prop)
-            (spred : Spred)
-            (p : @perm {x | interp_spred spred x})
-            (Q : R1 -> R2 -> Perms2) :
-    itree (sceE config) R1 ->
-    config ->
-    itree (sceE specConfig) R2 ->
-    specConfig ->
-    Prop :=
-  | bisim_gen_ret r1 c1 r2 c2 (Hspred : interp_spred spred (c1, c2)):
-      pre p (exist _ (c1, c2) Hspred) ->
-      in_Perms2 (Q r1 r2) p ->
-      bisim_gen bisim spred p Q (Ret r1) c1 (Ret r2) c2
-  | bisim_gen_err t1 c1 c2 :
-      bisim_gen bisim spred p Q t1 c1 (throw tt) c2
-  | bisim_gen_tau_L t1 c1 t2 c2 (Hspred : interp_spred spred (c1, c2)) :
-      pre p (exist _ (c1, c2) Hspred) ->
-      bisim_gen bisim spred p Q t1 c1 t2 c2 ->
-      bisim_gen bisim spred p Q (Tau t1) c1 t2 c2
-  | bisim_gen_tau_R t1 c1 t2 c2 (Hspred : interp_spred spred (c1, c2)) :
-      pre p (exist _ (c1, c2) Hspred) ->
-      bisim_gen bisim spred p Q t1 c1 t2 c2 ->
-      bisim_gen bisim spred p Q t1 c1 (Tau t2) c2
-  | bisim_gen_tau t1 c1 t2 c2 (Hspred : interp_spred spred (c1, c2)) :
-      pre p (exist _ (c1, c2) Hspred) ->
-      bisim spred p Q t1 c1 t2 c2 ->
-      bisim_gen bisim spred p Q (Tau t1) c1 (Tau t2) c2
-  | bisim_gen_modify_L (spred' : Spred)
-                       (Hspred' : forall x, interp_spred spred' x -> interp_spred spred x)
-                       (f : config -> config) k c1 t2 c2
-                       (p' : perm)
-                       (Hspred : interp_spred spred (c1, c2))
-                       (Hf : interp_spred spred' (f c1, c2)) :
-      pre p (exist _ (c1, c2) Hspred) ->
-      guar p (exist _ (c1, c2) Hspred) (exist _ (f c1, c2) (Hspred' _ Hf)) ->
-      sep_step _ _ _ Hspred' p p' ->
-      bisim_gen bisim spred' p' Q (k c1) (f c1) t2 c2 ->
-      bisim_gen bisim spred p Q (vis (Modify f) k) c1 t2 c2
-  | bisim_gen_modify_R (spred' : Spred)
-                        (Hspred' : forall x, interp_spred spred' x -> interp_spred spred x)
-                        t1 c1 f k c2 p'
-                        (Hspred : interp_spred spred (c1, c2))
-                        (Hf : interp_spred spred' (c1, f c2)):
-      pre p (exist _ (c1, c2) Hspred) ->
-      guar p (exist _ (c1, c2) Hspred) (exist _ (c1, f c2) (Hspred' _ Hf)) ->
-      sep_step _ _ _ Hspred' p p' ->
-      bisim_gen bisim spred' p' Q t1 c1 (k c2) (f c2) ->
-      bisim_gen bisim spred p Q t1 c1 (vis (Modify f) k) c2
-  | bisim_gen_modify (spred' : Spred)
-                      (Hspred' : forall x, interp_spred spred' x -> interp_spred spred x)
-                      f1 k1 c1 f2 k2 c2 p'
-                      (Hspred : interp_spred spred (c1, c2))
-                      (Hf : interp_spred spred' (f1 c1, f2 c2)) :
-      pre p (exist _ (c1, c2) Hspred) ->
-      guar p (exist _ (c1, c2) Hspred) (exist _ (f1 c1, f2 c2) (Hspred' _ Hf)) ->
-      sep_step _ _ _ Hspred' p p' ->
-      bisim spred' p' Q (k1 c1) (f1 c1) (k2 c2) (f2 c2) ->
-      bisim_gen bisim spred p Q (vis (Modify f1) k1) c1 (vis (Modify f2) k2) c2
-  | bisim_gen_choice_L k c1 t2 c2 (Hspred : interp_spred spred (c1, c2)) :
-      pre p (exist _ (c1, c2) Hspred) ->
-      (* sep_step p p' -> *)
-      (forall b, bisim_gen bisim spred p Q (k b) c1 t2 c2) ->
-      bisim_gen bisim spred p Q (vis Or k) c1 t2 c2
-  | bisim_gen_choice_R t1 c1 k c2 (Hspred : interp_spred spred (c1, c2)) :
-      pre p (exist _ (c1, c2) Hspred) ->
-      (* sep_step p p' -> *)
-      (forall b, bisim_gen bisim spred p Q t1 c1 (k b) c2) ->
-      bisim_gen bisim spred p Q t1 c1 (vis Or k) c2
-  | bisim_gen_choice k1 c1 k2 c2 (Hspred : interp_spred spred (c1, c2)):
-      pre p (exist _ (c1, c2) Hspred) ->
-      (* sep_step p p' -> *)
-      (forall b1, exists b2, bisim spred p Q (k1 b1) c1 (k2 b2) c2) ->
-      (forall b2, exists b1, bisim spred p Q (k1 b1) c1 (k2 b2) c2) ->
-      bisim_gen bisim spred p Q (vis Or k1) c1 (vis Or k2) c2
+  Inductive sbuter_gen {R1 R2 : Type} (sbuter : perm -> (R1 -> R2 -> Perms) -> itree (sceE config) R1 -> config -> itree (sceE specConfig) R2 -> specConfig -> Prop)
+            (p : perm) (Q : R1 -> R2 -> Perms) :
+    itree (sceE config) R1 -> config -> itree (sceE specConfig) R2 -> specConfig -> Prop :=
+  | sbuter_gen_ret r1 c1 r2 c2 :
+    pre p (c1, c2) ->
+    inv p (c1, c2) ->
+    p ∈ Q r1 r2 ->
+    sbuter_gen sbuter p Q (Ret r1) c1 (Ret r2) c2
+  | sbuter_gen_err t1 c1 c2 :
+      sbuter_gen sbuter p Q t1 c1 (throw tt) c2
+
+  | sbuter_gen_tau_L t1 c1 t2 c2 :
+    pre p (c1, c2) ->
+    inv p (c1, c2) ->
+    sbuter_gen sbuter p Q t1 c1 t2 c2 ->
+    sbuter_gen sbuter p Q (Tau t1) c1 t2 c2
+  | sbuter_gen_tau_R t1 c1 t2 c2 :
+    pre p (c1, c2) ->
+    inv p (c1, c2) ->
+    sbuter_gen sbuter p Q t1 c1 t2 c2 ->
+    sbuter_gen sbuter p Q t1 c1 (Tau t2) c2
+  | sbuter_gen_tau t1 c1 t2 c2 :
+    pre p (c1, c2) ->
+    inv p (c1, c2) ->
+    sbuter p Q t1 c1 t2 c2 ->
+    sbuter_gen sbuter p Q (Tau t1) c1 (Tau t2) c2
+
+  | sbuter_gen_modify_L f k c1 t2 c2 p' :
+    pre p (c1, c2) ->
+    inv p (c1, c2) ->
+    guar p (c1, c2) (f c1, c2) ->
+    sep_step p p' ->
+    sbuter_gen sbuter p' Q (k c1) (f c1) t2 c2 ->
+    sbuter_gen sbuter p Q (vis (Modify f) k) c1 t2 c2
+  | sbuter_gen_modify_R t1 c1 f k c2 p' :
+    pre p (c1, c2) ->
+    inv p (c1, c2) ->
+    guar p (c1, c2) (c1, f c2) ->
+    sep_step p p' ->
+    sbuter_gen sbuter p' Q t1 c1 (k c2) (f c2) ->
+    sbuter_gen sbuter p Q t1 c1 (vis (Modify f) k) c2
+  | sbuter_gen_modify f1 k1 c1 f2 k2 c2 p' :
+    pre p (c1, c2) ->
+    inv p (c1, c2) ->
+    guar p (c1, c2) (f1 c1, f2 c2) ->
+    sep_step p p' ->
+    sbuter p' Q (k1 c1) (f1 c1) (k2 c2) (f2 c2) ->
+    sbuter_gen sbuter p Q (vis (Modify f1) k1) c1 (vis (Modify f2) k2) c2
+
+  | sbuter_gen_choice_L k c1 t2 c2 p' :
+    pre p (c1, c2) ->
+    inv p (c1, c2) ->
+    sep_step p p' ->
+    (forall b, sbuter_gen sbuter p' Q (k b) c1 t2 c2) ->
+    sbuter_gen sbuter p Q (vis Or k) c1 t2 c2
+  | sbuter_gen_choice_R t1 c1 k c2 p' :
+    pre p (c1, c2) ->
+    inv p (c1, c2) ->
+    sep_step p p' ->
+    (forall b, sbuter_gen sbuter p' Q t1 c1 (k b) c2) ->
+    sbuter_gen sbuter p Q t1 c1 (vis Or k) c2
+  | sbuter_gen_choice k1 c1 k2 c2 p' :
+    pre p (c1, c2) ->
+    inv p (c1, c2) ->
+    sep_step p p' ->
+    (forall b1, exists b2, sbuter p' Q (k1 b1) c1 (k2 b2) c2) ->
+    (forall b2, exists b1, sbuter p' Q (k1 b1) c1 (k2 b2) c2) ->
+    sbuter_gen sbuter p Q (vis Or k1) c1 (vis Or k2) c2
   .
 
-  Lemma bisim_gen_mon {R1 R2} : monotone7 (@bisim_gen R1 R2).
+  Lemma sbuter_gen_mon {R1 R2} : monotone6 (@sbuter_gen R1 R2).
   Proof.
     repeat intro. induction IN; subst; try solve [econstructor; eauto]; auto.
     econstructor 11; eauto; intros.
-    - destruct (H0 b1). eexists; eauto.
-    - destruct (H1 b2). eexists; eauto.
+    - destruct (H2 b1). eexists; eauto.
+    - destruct (H3 b2). eexists; eauto.
   Qed.
-  #[local] Hint Resolve bisim_gen_mon : paco.
+  #[local] Hint Resolve sbuter_gen_mon : paco.
 
-  Definition bisim {R1 R2} := paco7 (@bisim_gen R1 R2) bot7.
+  Definition sbuter {R1 R2} := paco6 (@sbuter_gen R1 R2) bot6.
 
-  Lemma bisim_gen_pre {R1 R2} spred r p (Q : R1 -> R2 -> Perms2) t s c1 c2 Hspred :
-    bisim_gen r spred p Q t c1 s c2 ->
-    s = throw tt \/ pre p (exist _ (c1, c2) Hspred).
+  Lemma sbuter_gen_pre_inv {R1 R2} r p (Q : R1 -> R2 -> Perms) t s c1 c2 :
+    sbuter_gen r p Q t c1 s c2 ->
+    s = throw tt \/ (pre p (c1, c2) /\ inv p (c1, c2)).
   Proof.
-    inversion 1; subst; eauto; erewrite (proof_irrelevance _ Hspred); eauto.
+    inversion 1; auto.
   Qed.
 
-  Lemma bisim_lte {R1 R2} spred p Q Q' (t : itree (sceE config) R1) (s : itree (sceE specConfig) R2) c1 c2 :
-    bisim spred p Q t c1 s c2 ->
-    (forall r1 r2, (Q' r1 r2) ⊑2 (Q r1 r2)) ->
-    bisim spred p Q' t c1 s c2.
+  Lemma sbuter_lte {R1 R2} p Q Q' (t : itree (sceE config) R1) (s : itree (sceE specConfig) R2) c1 c2 :
+    sbuter p Q t c1 s c2 -> (forall r1 r2, Q r1 r2 ⊨ Q' r1 r2) -> sbuter p Q' t c1 s c2.
   Proof.
-    revert spred p Q Q' t s c1 c2. pcofix CIH. intros spred p Q Q' t s c1 c2 Htyping Hlte.
+    revert p Q Q' t s c1 c2. pcofix CIH. intros p Q Q' t s c1 c2 Htyping Hlte.
     punfold Htyping. pstep.
     induction Htyping; pclearbot; try solve [econstructor; eauto].
-    - econstructor; eauto. apply Hlte. auto.
+    - constructor; eauto. apply Hlte. auto.
     - econstructor 11; eauto; intros.
-      + destruct (H0 b1). eexists. right. eapply CIH; eauto. pclearbot. apply H2.
-      + destruct (H1 b2). eexists. right. eapply CIH; eauto. pclearbot. apply H2.
+      + destruct (H2 b1). eexists. right. eapply CIH; eauto. pclearbot. apply H4.
+      + destruct (H3 b2). eexists. right. eapply CIH; eauto. pclearbot. apply H4.
   Qed.
+
 
   (*
   Lemma bisim_spred_lte {R1 R2} (spred spred' : config * specConfig -> Prop) p Q
@@ -244,24 +226,20 @@ Section bisim.
   (* section variable: the spred lang and the interp function *)
   (** * Typing *)
   Definition typing {R1 R2} P Q (t : itree (sceE config) R1) (s : itree (sceE specConfig) R2) :=
-    (* forall "spreds" in the lang, apply interp to it *)
-    forall spred (p : @perm {x | interp_spred spred x}) c1 c2 (Hspred : (interp_spred spred) (c1, c2)),
-      in_Perms2 P p ->
-      pre p (exist _ (c1, c2) Hspred) ->
-      bisim spred p Q t c1 s c2.
+    forall p c1 c2, p ∈ P -> pre p (c1, c2) -> inv p (c1, c2) -> sbuter p Q t c1 s c2.
 
   Lemma typing_lte {R1 R2} P P' Q Q' (t : itree (sceE config) R1) (s : itree (sceE specConfig) R2) :
     typing P Q t s ->
-    P ⊑2 P' ->
-    (forall r1 r2, (Q' r1 r2) ⊑2 (Q r1 r2)) ->
+    P' ⊨ P ->
+    (forall r1 r2, Q r1 r2 ⊨ Q' r1 r2) ->
     typing P' Q' t s.
   Proof.
     repeat intro.
-    eapply bisim_lte; eauto.
+    eapply sbuter_lte; eauto.
   Qed.
 
   Lemma typing_ret {R1 R2} P Q (r1 : R1) (r2 : R2) :
-    (Q r1 r2) ⊑2 P -> typing P Q (Ret r1) (Ret r2).
+    P ⊨ (Q r1 r2) -> typing P Q (Ret r1) (Ret r2).
   Proof.
     repeat intro. pstep. econstructor; eauto.
   Qed.
@@ -283,89 +261,87 @@ Section bisim.
   Qed.
 
   Lemma typing_top {R1 R2} Q (t : itree (sceE config) R1) (s : itree (sceE specConfig) R2) :
-    typing top_Perms2 Q t s.
+    typing top_Perms Q t s.
   Proof.
     repeat intro. inversion H.
   Qed.
 
-  Lemma bisim_bottom {R1 R2} spred p Q (t : itree (sceE config) R1) (s : itree (sceE specConfig) R2) c1 c2:
-    bisim spred p Q t c1 s c2 -> bisim spred p (fun _ _ => bottom_Perms2) t c1 s c2.
+  Lemma sbuter_bottom {R1 R2} p Q (t : itree (sceE config) R1) (s : itree (sceE specConfig) R2) c1 c2:
+    sbuter p Q t c1 s c2 -> sbuter p (fun _ _ => bottom_Perms) t c1 s c2.
   Proof.
-    revert spred p Q t s c1 c2. pcofix CIH. intros. pstep. punfold H0.
+    revert p Q t s c1 c2. pcofix CIH. intros. pstep. punfold H0.
     induction H0; pclearbot; try solve [econstructor; simpl; eauto].
     econstructor 11; eauto; intros.
-    - destruct (H0 b1). eexists. right. eapply CIH; pclearbot. apply H2.
-    - destruct (H1 b2). eexists. right. eapply CIH; pclearbot; apply H2.
+    - destruct (H2 b1). eexists. right. eapply CIH; pclearbot; apply H4.
+    - destruct (H3 b2). eexists. right. eapply CIH; pclearbot; apply H4.
   Qed.
 
   Lemma typing_bottom {R1 R2} P Q (t : itree (sceE config) R1) (s : itree (sceE specConfig) R2) :
-    typing P Q t s -> typing P (fun _ _ => bottom_Perms2) t s.
+    typing P Q t s -> typing P (fun _ _ => bottom_Perms) t s.
   Proof.
-    repeat intro. eapply bisim_bottom; eauto.
+    repeat intro. eapply sbuter_bottom; eauto.
   Qed.
 
-  Lemma bisim_bind {R1 R2 S1 S2} spred (p : perm)
-        (Q : R1 -> S1 -> Perms2) (R : R2 -> S2 -> Perms2)
+  Lemma sbuter_bind {R1 R2 S1 S2} (p : perm) (Q : R1 -> S1 -> Perms) (R : R2 -> S2 -> Perms)
         (t1 : itree (sceE config) R1) (t2 : R1 -> itree (sceE config) R2)
         (s1 : itree (sceE specConfig) S1) (s2 : S1 -> itree (sceE specConfig) S2)
-        c1 c2 Hspred r :
-    pre p (exist _ (c1, c2) Hspred) ->
-    bisim spred p Q t1 c1 s1 c2 ->
-    (forall r1 r2 c1 c2 spred' Hspred' q,
-        in_Perms2 (Q r1 r2) q ->
-        pre q (exist _ (c1, c2) Hspred') ->
-        paco7 bisim_gen r spred' q R (t2 r1) c1 (s2 r2) c2) ->
-    paco7 bisim_gen r spred p R (x <- t1 ;; t2 x) c1 (x <- s1 ;; s2 x) c2.
+        c1 c2 r :
+    pre p (c1, c2) ->
+    inv p (c1, c2) ->
+    sbuter p Q t1 c1 s1 c2 ->
+    (forall r1 r2 p c1 c2, p ∈ (Q r1 r2) ->
+                      pre p (c1, c2) ->
+                      inv p (c1, c2) ->
+                      paco6 sbuter_gen r p R (t2 r1) c1 (s2 r2) c2) ->
+    paco6 sbuter_gen r p R (x <- t1 ;; t2 x) c1 (x <- s1 ;; s2 x) c2.
   Proof.
-    revert spred p Q R t1 t2 s1 s2 c1 c2 Hspred. pcofix CIH.
-    intros spred p Q R t1 t2 s1 s2 c1 c2 Hspred Hpre Htyping1 Htyping2.
+    revert p Q R t1 t2 s1 s2 c1 c2. pcofix CIH.
+    intros p Q R t1 t2 s1 s2 c1 c2 Hpre Hinv Htyping1 Htyping2.
     punfold Htyping1. induction Htyping1.
-    - do 2 rewritebisim @bind_ret_l. specialize (Htyping2 _ _ c1 c2 spred Hspred0 _ H0 H).
-      eapply paco7_mon; eauto.
+    - do 2 rewritebisim @bind_ret_l. specialize (Htyping2 _ _ _ c1 c2 H1 H H0).
+      eapply paco6_mon; eauto.
     - rewrite throw_bind. pstep. constructor.
     - rewritebisim @bind_tau.
-      specialize (IHHtyping1 _ Hpre Htyping2). punfold IHHtyping1.
-      pstep. econstructor; eauto.
+      specialize (IHHtyping1 Hpre Hinv Htyping2). punfold IHHtyping1.
+      pstep. constructor; auto.
     - rewritebisim @bind_tau.
-      specialize (IHHtyping1 _ Hpre Htyping2). punfold IHHtyping1.
-      pstep. econstructor; eauto.
+      specialize (IHHtyping1 Hpre Hinv Htyping2). punfold IHHtyping1.
+      pstep. constructor; auto.
     - do 2 rewritebisim @bind_tau. pclearbot.
-      pstep. econstructor 5; eauto.
-    - rewritebisim @bind_vis. eapply bisim_gen_pre in Htyping1. destruct Htyping1; subst.
+      pstep. constructor 5; auto. right. eapply CIH; eauto.
+    - rewritebisim @bind_vis. apply sbuter_gen_pre_inv in Htyping1.
+      destruct Htyping1 as [? | [? ?]]; subst.
       + rewrite throw_bind. pstep. constructor.
-      + pstep. econstructor; eauto. specialize (IHHtyping1 _ H2 Htyping2).
-        punfold IHHtyping1.
-    - rewritebisim @bind_vis. eapply bisim_gen_pre in Htyping1. destruct Htyping1; subst.
-      + pstep. econstructor; eauto. rewrite H2. rewrite throw_bind. constructor.
-      + pstep. econstructor; eauto. specialize (IHHtyping1 _ H2 Htyping2).
-        punfold IHHtyping1.
+      + specialize (IHHtyping1 H3 H4 Htyping2). punfold IHHtyping1. pstep. econstructor; eauto.
+    - rewritebisim @bind_vis. apply sbuter_gen_pre_inv in Htyping1.
+      destruct Htyping1 as [? | [? ?]]; subst.
+      + pstep. econstructor; eauto. rewrite H3. rewrite throw_bind. constructor.
+      + specialize (IHHtyping1 H3 H4 Htyping2). punfold IHHtyping1. pstep. econstructor; eauto.
     - do 2 rewritebisim @bind_vis. pclearbot.
-      pose proof H2. punfold H2.
+      pose proof H3. punfold H3.
       pstep. econstructor 8; eauto.
-      eapply bisim_gen_pre in H2. destruct H2; eauto.
-      left. pstep. rewrite H2. rewrite throw_bind. constructor.
+      destruct (sbuter_gen_pre_inv _ _ _ _ _ _ _ H3) as [? | [? ?]]; eauto.
+      rewrite H5. rewrite throw_bind. left. pstep. constructor.
     - rewritebisim @bind_vis. pstep. econstructor; eauto. intros.
-      specialize (H0 b). eapply bisim_gen_pre in H0. destruct H0.
-      + rewrite H0. rewrite throw_bind. constructor.
-      + specialize (H1 b _ H0 Htyping2). punfold H1.
+      destruct (sbuter_gen_pre_inv _ _ _ _ _ _ _ (H2 b)) as [? | [? ?]].
+      + rewrite H4. rewrite throw_bind. constructor.
+      + specialize (H3 b H4 H5 Htyping2). punfold H3.
     - rewritebisim @bind_vis. pstep. econstructor; eauto. intros.
-      specialize (H0 b). eapply bisim_gen_pre in H0. destruct H0.
-      + rewrite H0. rewrite throw_bind. constructor.
-      + specialize (H1 b _ H0 Htyping2). punfold H1.
+      destruct (sbuter_gen_pre_inv _ _ _ _ _ _ _ (H2 b)) as [? | [? ?]].
+      + rewrite H4. rewrite throw_bind. constructor.
+      + specialize (H3 b H4 H5 Htyping2). punfold H3.
     - do 2 rewritebisim @bind_vis. pclearbot. pstep. econstructor 11; eauto; intros.
-      + specialize (H0 b1). destruct H0. pclearbot.
-        punfold H0. pose proof H0. eapply bisim_gen_pre in H0. destruct H0.
-        * exists x. left. pstep. rewrite H0. rewrite throw_bind. econstructor; eauto.
+      + specialize (H2 b1). destruct H2. pclearbot.
+        punfold H2. destruct (sbuter_gen_pre_inv _ _ _ _ _ _ _ H2) as [? | [? ?]].
+        * exists x. left. pstep. rewrite H4. rewrite throw_bind. econstructor; eauto.
         * eexists. right. eapply CIH; eauto. pstep; eauto.
-      + specialize (H1 b2). destruct H1. pclearbot.
-        punfold H1. pose proof H1. eapply bisim_gen_pre in H1. destruct H1.
-        * exists x. left. pstep. rewrite H1. rewrite throw_bind. econstructor; eauto.
+      + specialize (H3 b2). destruct H3. pclearbot.
+        punfold H3. destruct (sbuter_gen_pre_inv _ _ _ _ _ _ _ H3) as [? | [? ?]].
+        * exists x. left. pstep. rewrite H4. rewrite throw_bind. econstructor; eauto.
         * eexists. right. eapply CIH; eauto. pstep; eauto.
-
-          Unshelve. all: eauto.
   Qed.
 
-  Lemma typing_bind {R1 R2 S1 S2} (P : Perms2) (Q : R1 -> S1 -> Perms2) (R : R2 -> S2 -> Perms2)
+  Lemma typing_bind {R1 R2 S1 S2} (P : Perms) (Q : R1 -> S1 -> Perms) (R : R2 -> S2 -> Perms)
         (t1 : itree (sceE config) R1) (t2 : R1 -> itree (sceE config) R2)
         (s1 : itree (sceE specConfig) S1) (s2 : S1 -> itree (sceE specConfig) S2) :
     typing P Q t1 s1 ->
@@ -373,8 +349,164 @@ Section bisim.
     typing P R (x <- t1 ;; t2 x) (x <- s1 ;; s2 x).
   Proof.
     repeat intro.
-    eapply bisim_bind; eauto.
-    intros. eapply H0; eauto.
+    eapply sbuter_bind; eauto.
+  Qed.
+
+  Lemma sbuter_frame {R1 R2} p r p' Q R (t : itree (sceE config) R1) (s : itree (sceE specConfig) R2) c1 c2:
+    pre p' (c1, c2) ->
+    inv p' (c1, c2) ->
+    r ∈ R ->
+    p ** r <= p' ->
+    sbuter p Q t c1 s c2 ->
+    sbuter p' (fun r1 r2 => Q r1 r2 * R) t c1 s c2.
+  Proof.
+    revert p r p' Q R t s c1 c2. pcofix CIH. rename r into r0.
+    intros p r p' Q R t s c1 c2 Hpre Hinv Hr Hlte Hsbuter. pstep. punfold Hsbuter.
+    revert p' Hlte Hpre Hinv. generalize dependent r.
+    induction Hsbuter; intros; pclearbot; try solve [econstructor; eauto].
+    - constructor; auto. eapply Perms_upwards_closed; eauto.
+      do 2 eexists. split; [| split; [| split]]; eauto.
+      (* apply Hlte in Hpre. apply Hpre. *)
+      reflexivity.
+      eapply inv_inc in Hinv; eauto. apply Hinv.
+    - apply sbuter_gen_pre_inv in Hsbuter.
+      destruct Hsbuter as [? | [? ?]]; [subst; constructor |].
+      constructor 6 with (p':= p' ** r ** invperm (inv  p'0)); eauto.
+      + apply Hlte; auto. constructor. left. auto.
+      + (* so p'0 has a stronger inv than p and r *)
+        (* so we want this evar to be p' ** r ** invperm p'0 *)
+        admit.
+        (* eapply sep_step_lte; eauto. apply sep_step_sep_conj_l; eauto. *)
+        (* apply Hlte in Hpre. apply Hpre. *)
+      + eapply IHHsbuter; eauto. admit. (* reflexivity. *)
+        {
+          split.
+          split; auto.
+          apply Hlte in Hpre. destruct Hpre as (? & ?). respects.
+          eapply inv_inc in Hinv; eauto. destruct Hinv as (? & ? & ?). apply H9; auto.
+
+          auto.
+
+          cbn. auto.
+        }
+        {
+          split; [| split]; auto.
+          - split; [| split]; auto. apply Hlte. apply Hinv.
+        * apply H1. apply Hlte in Hpre. apply Hpre.
+    - econstructor; eauto.
+      + apply Hlte. constructor. left. auto.
+      + eapply sep_step_lte; eauto. apply sep_step_sep_conj_l; eauto.
+        apply Hlte in Hpre. apply Hpre.
+      + apply sbuter_gen_pre in Hsbuter. destruct Hsbuter; [rewrite H2; constructor |].
+        eapply IHHsbuter; eauto. reflexivity.
+        split; [| split]; auto.
+        * apply Hlte in Hpre. destruct Hpre as (? & ? & ?). respects.
+          apply H5. auto.
+        * apply H1. apply Hlte in Hpre. apply Hpre.
+    - econstructor 8; eauto.
+      3: { pose proof H2 as Hsbuter.
+           punfold Hsbuter. apply sbuter_gen_pre in Hsbuter.
+           destruct Hsbuter; [rewrite H3; left; pstep; constructor |].
+           right. eapply CIH. 4: apply H2. 2: eauto. 2: reflexivity.
+           apply Hlte in Hpre. destruct Hpre as (? & ? & ?).
+           split; [| split]; auto.
+           respects. apply H6. auto.
+      }
+      + apply Hlte. constructor. left. auto.
+      + eapply sep_step_lte; eauto. apply sep_step_sep_conj_l; auto.
+        apply Hlte in Hpre. apply Hpre.
+    - econstructor; eauto.
+      + eapply sep_step_lte; eauto. apply sep_step_sep_conj_l; eauto.
+        apply Hlte in Hpre. apply Hpre.
+      + intros. specialize (H1 b).
+        apply sbuter_gen_pre in H1. destruct H1; [subst; constructor |].
+        eapply H2; eauto. reflexivity.
+        apply Hlte in Hpre. destruct Hpre as (? & ? & ?).
+        split; [| split]; auto.
+    - econstructor; eauto.
+      + eapply sep_step_lte; eauto. apply sep_step_sep_conj_l; eauto.
+        apply Hlte in Hpre. apply Hpre.
+      + intros. specialize (H1 b).
+        apply sbuter_gen_pre in H1. destruct H1; [rewrite H1; constructor |].
+        eapply H2; eauto. reflexivity.
+        apply Hlte in Hpre. destruct Hpre as (? & ? & ?).
+        split; [| split]; auto.
+    - econstructor 11; eauto.
+      2: { intros. specialize (H1 b1). destruct H1 as (b2 & H1). pclearbot. exists b2.
+           pose proof H1 as Hsbuter.
+           punfold Hsbuter. apply sbuter_gen_pre in Hsbuter.
+           destruct Hsbuter; [rewrite H3; left; pstep; constructor |].
+           right. eapply CIH. 4: apply H1. 2: eauto. 2: reflexivity.
+           apply Hlte in Hpre. destruct Hpre as (? & ? & ?).
+           split; [| split]; auto.
+      }
+      2: { intros. specialize (H2 b2). destruct H2 as (b1 & H2). pclearbot. exists b1.
+           pose proof H2 as Hsbuter.
+           punfold Hsbuter. apply sbuter_gen_pre in Hsbuter.
+           destruct Hsbuter; [rewrite H3; left; pstep; constructor |].
+           right. eapply CIH. 4: apply H2. 2: eauto. 2: reflexivity.
+           apply Hlte in Hpre. destruct Hpre as (? & ? & ?).
+           split; [| split]; auto.
+      }
+      eapply sep_step_lte; eauto. apply sep_step_sep_conj_l; auto.
+      apply Hlte in Hpre. apply Hpre.
+  Qed.
+
+
+  Lemma typing_frame {R1 R2} P Q R (t : itree (sceE config) R1) (s : itree (sceE specConfig) R2):
+    typing P Q t s ->
+    typing (P * R) (fun r1 r2 => Q r1 r2 * R) t s.
+  Proof.
+    intros Ht p' c1 c2 (p & r & Hp & Hr & Hlte & Hsep) Hpre Hinv.
+    assert (Hpre': forall x, pre p' x -> pre (p ** r) x) by admit.
+    destruct Hlte as [Hinv' Hsep_step]. red in Hinv'.
+    specialize (Ht p).
+    (* pose proof Hpre as H. apply Hlte in H. destruct H as (Hprep & Hprer & Hsep'). *)
+    (* eapply sbuter_frame; eauto. *)
+  Abort.
+
+  Lemma sbuter_frame' {R1 R2} p r Q R (t : itree (sceE config) R1) (s : itree (sceE specConfig) R2) c1 c2:
+    pre (p ** r) (c1, c2) ->
+    inv (p ** r) (c1, c2) ->
+    r ∈ R ->
+    sbuter p Q t c1 s c2 ->
+    sbuter (p ** r) (fun r1 r2 => Q r1 r2 * R) t c1 s c2.
+  Proof.
+    revert p r Q R t s c1 c2. pcofix CIH. rename r into r0.
+    intros p r Q R t s c1 c2 Hpre Hinv Hr Hsbuter. pstep. punfold Hsbuter.
+    revert Hr Hpre Hinv. generalize dependent r.
+    induction Hsbuter; intros; pclearbot; try solve [econstructor; eauto].
+    - constructor; auto.
+      apply sep_conj_Perms_perm; auto. apply Hinv.
+    - apply sbuter_gen_pre_inv in Hsbuter. destruct Hsbuter; [subst; constructor |].
+      destruct H3.
+      econstructor; eauto.
+      3: {
+        destruct Hinv as (Hinvp & Hinvr & Hsep).
+        eapply IHHsbuter; eauto.
+        * split; auto.
+          eapply pre_respects. apply Hsep; eauto. apply Hpre.
+        * split; [| split]; auto.
+          2: { apply H2. apply Hsep. }
+          eapply inv_rely; eauto. apply Hsep; eauto.
+      }
+      + constructor. left. auto.
+      + apply sep_step_frame; auto. apply Hinv.
+    -
+  Admitted.
+
+
+  Lemma sbuter_frame {R1 R2} p r p' Q R (t : itree (sceE config) R1) (s : itree (sceE specConfig) R2) c1 c2:
+    pre p' (c1, c2) ->
+    inv p' (c1, c2) ->
+    r ∈ R ->
+    p ⊥ r ->
+    sep_step p' (p ** r) ->
+    sbuter p Q t c1 s c2 ->
+    sbuter p' (fun r1 r2 => Q r1 r2 * R) t c1 s c2.
+  Proof.
+    intros. eapply sbuter_lte'; eauto.
+    apply sbuter_frame'; eauto. admit.
   Qed.
 
   Lemma restrict_rely C (spred spred' spred'' : C -> Prop) Hspred1 Hspred2
